ProvabilityLogic/Logic/Basic.lean
@@ -1,0 +1,13 @@
+module
+
+public import ProvabilityLogic.Hilbert.Basic
+public import ProvabilityLogic.Kripke.Cone
+
+@[expose]
+public section
+
+variable {α : Type u}
+
+abbrev Logic (α) := Set (Formula α)
+
+end
